Basic stub handler verification

pkvm_handler/wp.v
@@ -56,43 +56,56 @@
 Require Import isla.aarch64.aarch64.
 Require Import isla.examples.pkvm_handler.instrs.
 
+(*SPEC_START*)
+Definition pkvm_sys_regs' : list (reg_kind * valu_shape) := [
+  (KindReg "SCTLR_EL1" , ExactShape (RVal_Bits [BV{64} 0x0000000004000002] ));
+  (KindReg "SCR_EL3" , ExactShape (RVal_Bits [BV{32} 0x00000501] ));
+  (KindReg "TCR_EL1" , ExactShape (RVal_Bits [BV{64} 0] ));
+  (KindReg "TCR_EL2" , ExactShape (RVal_Bits [BV{64} 0] ));
+  (KindReg "HCR_EL2" , ExactShape (RVal_Bits [BV{64} 0x0000000080000000] ));
+  (KindReg "CFG_ID_AA64PFR0_EL1_EL0" , ExactShape (RVal_Bits [BV{4} 1] ));
+  (KindReg "CFG_ID_AA64PFR0_EL1_EL1" , ExactShape (RVal_Bits [BV{4} 1] ));
+  (KindReg "CFG_ID_AA64PFR0_EL1_EL2" , ExactShape (RVal_Bits [BV{4} 1] ));
+  (KindReg "CFG_ID_AA64PFR0_EL1_EL3" , ExactShape (RVal_Bits [BV{4} 1] ));
+  (KindReg "OSLSR_EL1" , ExactShape (RVal_Bits [BV{32} 0] ));
+  (KindReg "OSDLR_EL1" , ExactShape (RVal_Bits [BV{32} 0] ));
+  (KindReg "EDSCR" , ExactShape (RVal_Bits [BV{32} 0] ));
+  (KindReg "MPIDR_EL1" , ExactShape (RVal_Bits [BV{64} 0] ));
+  (KindReg "MDSCR_EL1" , ExactShape (RVal_Bits [BV{32} 0] ));
+  (KindReg "MDCR_EL2" , ExactShape (RVal_Bits [BV{32} 0] ));
+  (KindReg "MDCR_EL3" , ExactShape (RVal_Bits [BV{32} 0] ));
+  (KindField "PSTATE" "SP" , ExactShape (RVal_Bits [BV{1} 1] ));
+  (KindField "PSTATE" "nRW" , ExactShape (RVal_Bits [BV{1} 0] ));
+  (KindField "PSTATE" "D" , ExactShape (RVal_Bits [BV{1} 1]));
+  (KindReg "__isla_monomorphize_writes", ExactShape (RVal_Bool false));
+  (KindReg "__isla_monomorphize_reads", ExactShape (RVal_Bool false));
+  (KindReg "__highest_el_aarch32", ExactShape (RVal_Bool false));
+  (KindReg "__CNTControlBase", ExactShape (RVal_Bits [BV{52} 0]));
+  (KindReg "__v85_implemented", ExactShape (RVal_Bool false));
+  (KindReg "__v84_implemented", ExactShape (RVal_Bool false));
+  (KindReg "__v83_implemented", ExactShape (RVal_Bool false));
+  (KindReg "__v82_implemented", ExactShape (RVal_Bool false));
+  (KindReg "__v81_implemented", ExactShape (RVal_Bool true));
+  (KindReg "__trickbox_enabled", ExactShape (RVal_Bool false))
+].
+
+Definition pkvm_sys_regs := 
+  (KindReg "SCTLR_EL2", ExactShape (RVal_Bits [BV{64} 0x4000002])) :: 
+  (KindField "PSTATE" "EL" , ExactShape (RVal_Bits [BV{2} 2] )) ::
+  pkvm_sys_regs'.
+Definition pkvm_sys_regs_updated :=
+  (KindReg "SCTLR_EL2", ExactShape (RVal_Bits [BV{64} 0x4000000])) ::
+  (KindField "PSTATE" "EL" , ExactShape (RVal_Bits [BV{2} 2] )) ::
+  pkvm_sys_regs'.
+Definition pkvm_eret_sys_regs :=
+  (KindReg "SCTLR_EL2", ExactShape (RVal_Bits [BV{64} 0x4000002])) :: 
+  (KindField "PSTATE" "EL" , ExactShape (RVal_Bits [BV{2} 1] )) ::
+  pkvm_sys_regs'.
+(*SPEC_END*)
+
 Definition instrs_iprop `{!islaG Σ} `{!threadG} := ([∗ list] i ∈ instr_map, instr i.1 (Some i.2))%I.
 
-(*PROOF_START*)
-Definition spec_stp `{!islaG Σ} `{!threadG} a sp : iProp Σ :=
-    ∃ (vold1 vold2 v v': bv 64),
-    "R0" ↦ᵣ RVal_Bits v ∗
-    "R1" ↦ᵣ RVal_Bits v' ∗
-    (bv_unsigned sp - 16) ↦ₘ vold1 ∗
-    (bv_unsigned sp - 8) ↦ₘ vold2 ∗
-    ⌜bv_unsigned sp < 2 ^ 52⌝ ∗
-    ⌜bv_unsigned sp > 16⌝ ∗
-    ⌜bv_unsigned sp `mod` 8 = 0⌝ ∗
-    "SP_EL2" ↦ᵣ RVal_Bits sp ∗
-    reg_col sys_regs ∗
-    instr_pre a (
-      "R0" ↦ᵣ RVal_Bits v ∗
-      "R1" ↦ᵣ RVal_Bits v' ∗
-      "SP_EL2" ↦ᵣ RVal_Bits (bv_sub sp [BV{64} 16])∗
-      reg_col sys_regs ∗
-      (bv_unsigned sp - 16) ↦ₘ v ∗
-      (bv_unsigned sp - 8) ↦ₘ v' ∗
-      True).
 
-Lemma stp_wp `{!islaG Σ} `{!threadG} (sp : bv 64) :
-  instr 0x7400 (Some a7400) -∗
-  instr_body 0x7400 (spec_stp 0x7404 sp).
-Proof.
-  iStartProof.
-  unfold spec_stp.
-  unfold instrs_iprop.
-  simpl.
-  liARun.
-  Unshelve.
-  all: try (repeat f_equal; bv_solve).
-  all: prepare_sidecond; bv_solve.
-Time Qed.
-(*PROOF_END*)
 
 (*SPEC_START*)
 Definition mrs_regs_32 :=
@@ -115,72 +128,140 @@ Definition exists_reg r :=
   [(KindReg r, BitsShape 64)].
 (*SPEC_END*)
 
-(*PROOF_START*)
-Definition spec_mrs `{!islaG Σ} `{!threadG} a (vold : bv 32) (v : bv 64) x : iProp Σ :=
-  reg_col mrs_regs_32 ∗
-  reg_col mrs_regs_64 ∗
-  reg_col (exists_reg "R0") ∗
-  reg_col sys_regs ∗
-  "ESR_EL2" ↦ᵣ RVal_Bits vold ∗
-  ⌜bv_unsigned vold = x⌝ ∗
-  ⌜bv_unsigned v = x⌝ ∗
-  instr_pre a (
-    reg_col sys_regs ∗
-    "R0" ↦ᵣ RVal_Bits v ∗
-    True
-  ).
-
-Lemma mrs_wp `{!islaG Σ} `{!threadG} (vold: bv 32) (v : bv 64) x :
-  instr 0x7404 (Some a7404) -∗
-  instr_body 0x7404 (spec_mrs 0x7408 vold v x).
-Proof.
-  iStartProof.
-  unfold spec_mrs.
-  unfold exists_reg.
-  liARun.
-  Unshelve.
-  (* TODO: Check if bv_solve on the latest branch solves this, otherwise fix it *)
-  all: prepare_sidecond.
-  bv_solve.
-Time Qed.
-
-Definition spec_lsr `{!islaG Σ} `{!threadG} a (v vold : bv 64) : iProp Σ :=
-  "R0" ↦ᵣ RVal_Bits vold ∗
-  ⌜bv_unsigned v = Z.shiftr (bv_unsigned vold) 26⌝ ∗
-  reg_col sys_regs ∗
-  instr_pre a (
-    reg_col sys_regs ∗
-    "R0" ↦ᵣ RVal_Bits v ∗
-    True
-  ).
-
-Lemma lsr_wp `{!islaG Σ} `{!threadG} (v vold : bv 64):
-  instr 0x7408 (Some a7408) -∗
-  instr_body 0x7408 (spec_lsr 0x740c v vold).
-Proof.
-  iStartProof.
-  unfold spec_lsr.
-  liARun.
-  Unshelve.
-  all: prepare_sidecond.
-  by bits_simplify.
-Time Qed.
-(*PROOF_END*)
-
 (*SPEC_START*)
-Definition spec `{!islaG Σ} `{!threadG} (sp stub_handler_addr offset: bv 64) (esr : bv 32) : iProp Σ :=
-  ∃ v0 v1 v5 v6: bv 64,
-  reg_col sys_regs ∗
+Definition rest_of_pstate : list (reg_kind * valu_shape) := [
+  (KindField "PSTATE" "F"    , BitsShape 1);
+  (KindField "PSTATE" "I"    , BitsShape 1);
+  (KindField "PSTATE" "A"    , BitsShape 1);
+  (KindField "PSTATE" "D"    , ExactShape (RVal_Bits [BV{1} 1]));
+  (KindField "PSTATE" "BTYPE", BitsShape 2);
+  (KindField "PSTATE" "SBSS" , BitsShape 1);
+  (KindField "PSTATE" "IL"   , BitsShape 1);
+  (KindField "PSTATE" "SS"   , BitsShape 1);
+  (KindField "PSTATE" "PAN"  , BitsShape 1);
+  (KindField "PSTATE" "UAO"  , BitsShape 1);
+  (KindField "PSTATE" "DIT"  , BitsShape 1);
+  (KindField "PSTATE" "TCO"  , BitsShape 1)
+].
+
+Definition reset_spec `{!islaG Σ} `{!threadG} : iProp Σ :=
+  ∃ (elr : bv 64) (spsr : bv 32),
+  reg_col pkvm_sys_regs ∗
   reg_col mrs_regs ∗
   reg_col CNVZ_regs ∗
-  (* Move to sys_regs *)
+  reg_col rest_of_pstate ∗
+  reg_col [
+    (KindReg "R5", BitsShape 64);
+    (KindReg "R6", BitsShape 64);
+    (KindReg "VBAR_EL2", BitsShape 64);
+    (KindReg "EventRegister", BitsShape 1)
+  ] ∗
+  "SPSR_EL2" ↦ᵣ RVal_Bits spsr ∗
+  ⌜bv_extract 0  1 spsr = [BV{1} 1]⌝ ∗
+  ⌜bv_extract 1  1 spsr = [BV{1} 0]⌝ ∗
+  ⌜bv_extract 2  2 spsr = [BV{2} 2]⌝ ∗
+  ⌜bv_extract 4  1 spsr = [BV{1} 0]⌝ ∗
+  ⌜bv_extract 9  1 spsr = [BV{1} 1]⌝ ∗
+  ⌜bv_extract 20 1 spsr = [BV{1} 0]⌝ ∗ 
+  "ELR_EL2" ↦ᵣ RVal_Bits elr ∗
+  ⌜bv_extract 55 1 elr = [BV{1} 0]⌝ ∗
+  instr_body (bv_unsigned elr) (
+    (* sctlr is updated by this code, but we claim to know enough about its value that the update is trivial.
+       This should probably be relaxed
+    *)
+    reg_col pkvm_sys_regs_updated ∗
+    reg_col mrs_regs ∗
+    reg_col CNVZ_regs ∗
+    reg_col rest_of_pstate ∗
+    reg_col [
+      (KindReg "R5", BitsShape 64);
+      (KindReg "R6", BitsShape 64);
+      (KindReg "SPSR_EL2", BitsShape 32);
+      (KindReg "ELR_EL2", BitsShape 64);
+      (KindReg "EventRegister", BitsShape 1)
+    ] ∗
+    "VBAR_EL2" ↦ᵣ RVal_Bits [BV{64} 116632] ∗
+    True
+  ).
+
+  Definition stub_handler_spec `{!islaG Σ} `{!threadG} : iProp Σ :=
+    ∃ (b elr el2_cont: bv 64) (spsr : bv 32),
+    reg_col pkvm_sys_regs ∗
+    reg_col mrs_regs ∗
+    reg_col CNVZ_regs ∗
+    reg_col rest_of_pstate ∗
+    reg_col [(KindReg "EventRegister", BitsShape 1)] ∗
+    "R0" ↦ᵣ RVal_Bits b ∗
+    "R1" ↦ᵣ RVal_Bits el2_cont ∗
+    reg_col 
+      [
+        (KindReg "R2", BitsShape 64);
+        (KindReg "R3", BitsShape 64);
+        (KindReg "R4", BitsShape 64);
+        (KindReg "R5", BitsShape 64);
+        (KindReg "R6", BitsShape 64);
+        (KindReg "VBAR_EL2", BitsShape 64)
+      ] ∗
+    "SPSR_EL2" ↦ᵣ RVal_Bits spsr ∗
+    "ELR_EL2" ↦ᵣ RVal_Bits elr ∗
+    ⌜bv_extract 0  1 spsr = [BV{1} 1]⌝ ∗
+    ⌜bv_extract 1  1 spsr = [BV{1} 0]⌝ ∗
+    ⌜bv_extract 2  2 spsr = [BV{2} 1]⌝ ∗
+    ⌜bv_extract 4  1 spsr = [BV{1} 0]⌝ ∗
+    ⌜bv_extract 9  1 spsr = [BV{1} 1]⌝ ∗
+    ⌜bv_extract 20 1 spsr = [BV{1} 0]⌝ ∗ 
+    ⌜bv_extract 55 1 elr = [BV{1} 0]⌝ ∗
+    ⌜bv_extract 55 1 el2_cont = [BV{1} 0]⌝ ∗
+    (* We handle only two of the 3 hypercalls this handler supports for now*)
+    ⌜bv_unsigned b < 2⌝ ∗
+    instr_body (bv_unsigned el2_cont) (
+      (* There should be way more here, but eliding it for now as it doesn't affect the proof *)
+      ⌜bv_unsigned b = 1 ⌝ ∗
+      reg_col pkvm_sys_regs_updated ∗
+      reg_col CNVZ_regs ∗
+      "VBAR_EL2" ↦ᵣ RVal_Bits [BV{64} 116632] ∗
+      True
+    ) ∗
+    instr_body (bv_unsigned elr) (
+      "R0" ↦ᵣ RVal_Bits [BV{64} 0xbadca11] ∗
+      reg_col pkvm_eret_sys_regs ∗
+      reg_col CNVZ_regs ∗
+      True
+    ).
+
+Definition spec `{!islaG Σ} `{!threadG} (sp stub_handler_addr offset: bv 64) (esr : bv 32) : iProp Σ :=
+  ∃ (param el2_cont elr : bv 64) (spsr : bv 32),
+  reg_col pkvm_sys_regs ∗
+  reg_col mrs_regs ∗
+  reg_col CNVZ_regs ∗
+  reg_col rest_of_pstate ∗
+  reg_col [(KindReg "EventRegister", BitsShape 1)] ∗
+  reg_col [
+    (KindReg "R2", BitsShape 64);
+    (KindReg "R3", BitsShape 64);
+    (KindReg "R4", BitsShape 64);
+    (KindReg "R5", BitsShape 64);
+    (KindReg "R6", BitsShape 64)
+  ] ∗
+  reg_col [(KindReg "VBAR_EL2", BitsShape 64)] ∗
+  (* Move to pkvm_sys_regs *)
   "InGuardedPage" ↦ᵣ RVal_Bool false ∗
   "ESR_EL2" ↦ᵣ RVal_Bits esr ∗
-  "R0" ↦ᵣ RVal_Bits v0 ∗
-  "R1" ↦ᵣ RVal_Bits v1 ∗
-  "R5" ↦ᵣ RVal_Bits v5 ∗
-  "R6" ↦ᵣ RVal_Bits v6 ∗
+  "R0" ↦ᵣ RVal_Bits param ∗
+  "R1" ↦ᵣ RVal_Bits el2_cont ∗
   "SP_EL2" ↦ᵣ RVal_Bits sp ∗
+  "SPSR_EL2" ↦ᵣ RVal_Bits spsr ∗
+  "ELR_EL2" ↦ᵣ RVal_Bits elr ∗
+  ⌜bv_extract 0 1 spsr = [BV{1} 1]⌝ ∗
+  ⌜bv_extract 1 1 spsr = [BV{1} 0]⌝ ∗
+  ⌜bv_extract 2 2 spsr = [BV{2} 1]⌝ ∗
+  ⌜bv_extract 4 1 spsr = [BV{1} 0]⌝ ∗
+  ⌜bv_extract 9 1 spsr = [BV{1} 1]⌝ ∗
+  ⌜bv_extract 20 1 spsr = [BV{1} 0]⌝ ∗
+  ⌜bv_extract 55 1 elr = [BV{1} 0]⌝ ∗
+  ⌜bv_extract 55 1 el2_cont = [BV{1} 0]⌝ ∗
+  (* Don't handle this hypercall for now *)
+  ⌜bv_unsigned param ≠ 2⌝ ∗
   (bv_unsigned sp - 16) ↦ₘ? 8 ∗
   (bv_unsigned sp - 8) ↦ₘ? 8 ∗
   ⌜bv_unsigned sp < 2 ^ 52⌝ ∗
@@ -188,21 +269,33 @@ Definition spec `{!islaG Σ} `{!threadG} (sp stub_handler_addr offset: bv 64) (e
   ⌜bv_unsigned sp `mod` 8 = 0⌝ ∗
   0x77f8 ↦ₘ stub_handler_addr ∗
   (instr_pre 0x6800 (⌜Z.shiftr (bv_unsigned esr) 26 ≠ 22⌝ ∗ ∃ (v : bv 64), "R0" ↦ᵣ RVal_Bits v ∗ ⌜bv_unsigned v ≠ 22⌝ ∗ True) ∧
-  instr_pre 0x6800 (⌜Z.shiftr (bv_unsigned esr) 26 = 22⌝ ∗ ⌜Z.ge (bv_unsigned v0) 3⌝ ∗ True)) ∗
+  instr_pre 0x6800 (⌜Z.shiftr (bv_unsigned esr) 26 = 22⌝ ∗ ⌜Z.ge (bv_unsigned param) 3⌝ ∗ True)) ∗
   (* Possibly should handle that this address gets shifted (even if it's by zero in this code) *)
   instr_pre (bv_unsigned (bv_sub stub_handler_addr offset)) (
-    ⌜Z.shiftr (bv_unsigned esr) 26 = 22⌝ ∗
+    stub_handler_spec
+    (*⌜Z.shiftr (bv_unsigned esr) 26 = 22⌝ ∗
     ⌜Z.lt (bv_unsigned v0) 3⌝ ∗
     "SP_EL2" ↦ᵣ RVal_Bits sp ∗
     "R5" ↦ᵣ RVal_Bits (bv_sub stub_handler_addr offset)∗
     "R6" ↦ᵣ RVal_Bits offset ∗
-    True).
+    True*)) ∗
+  instr_body (bv_unsigned el2_cont) (
+    ⌜bv_unsigned param = 1⌝ ∗ reg_col pkvm_sys_regs_updated ∗
+    reg_col CNVZ_regs ∗
+    "VBAR_EL2" ↦ᵣ RVal_Bits [BV{64} 116632] ∗
+    True
+  ) ∗
+  instr_body (bv_unsigned elr) (
+    "R0" ↦ᵣ RVal_Bits [BV{64} 0xbadca11] ∗
+    reg_col pkvm_eret_sys_regs ∗
+    reg_col CNVZ_regs ∗
+    True
+  ).
 (*SPEC_END*)
 
 (* This is simpler than I was expecting, could probably write a tactic for these
    so they can be generated by the frontend *)
-
-(*PROOF_START*)
+(*SPEC_START*)
 Lemma a742c_spec `{!islaG Σ} `{!threadG} pc (b : bv 16):
   instr pc (Some (partial_trace (Val_Bits b) a742c)) -∗
   instr_body pc (movk_spec pc "R6" b 1).
@@ -251,15 +344,16 @@ Definition a7434_spec_inst `{!islaG Σ} `{!threadG} pc b :=
 Global Existing Instance a7434_spec_inst.
 
 Definition load_offset_spec `{!islaG Σ} `{!threadG} offset pc_cont : iProp Σ :=
-  ∃ v,
-  reg_col sys_regs ∗
-  "R6" ↦ᵣ v ∗
+  reg_col pkvm_sys_regs ∗
+  reg_col [(KindReg "R6", BitsShape 64)] ∗
   instr_body pc_cont (
-    reg_col sys_regs ∗
+    reg_col pkvm_sys_regs ∗
     "R6" ↦ᵣ RVal_Bits offset ∗
     True
   ).
+(*SPEC_END*)
 
+(*PROOF_START*)
 Lemma load_offset_verif `{!islaG Σ} `{!threadG} (offset : bv 64) :
   instr 29736 (Some (partial_trace (Val_Bits (bv_extract 0 16 offset)) a7428)) ∗
   instr 29740 (Some (partial_trace (Val_Bits (bv_extract 16 16 offset)) a742c)) ∗
@@ -278,7 +372,7 @@ Time Qed.
 
 Lemma wp `{!islaG Σ} `{!threadG} sp esr stub_handler_addr (offset : bv 64) :
   instr 29696 (Some a7400) ∗
-  instr 29700 (Some a7404) ∗
+  instr 29700 (Some a7404) ∗ 
   instr 29704 (Some a7408) ∗
   instr 29708 (Some a740c) ∗
   instr 29712 (Some a7410) ∗
@@ -306,19 +400,18 @@ Proof.
     liARun.
   + unfold load_offset_spec.
     liARun.
+    unfold stub_handler_spec.
+    liARun.
   Unshelve.
   all: prepare_sidecond.
   all: try bv_solve.
-  * contradict H4.
-    rewrite H3.
-    rewrite <- H4.
-    by bits_simplify.
-  * rewrite <- H4.
+  * contradict H13.
+    rewrite H12.
     assert(G: bv_unsigned (bv_concat 64 [BV{32} 0] esr) = bv_unsigned esr); [bv_solve|].
-    by rewrite G in H3.
-  * rewrite <- H4.
-    assert(G: bv_unsigned (bv_concat 64 [BV{32} 0] esr) = bv_unsigned esr); [bv_solve|].
-    by rewrite G in H3.
+    by rewrite G.
+  * assert(G: bv_unsigned (bv_concat 64 [BV{32} 0] esr) = bv_unsigned esr); [bv_solve|].
+    rewrite G in H12.
+    by rewrite <- H12.
 (*PROOF_END*)
 Time Qed.
 
@@ -341,9 +434,99 @@ Lemma wp' `{!islaG Σ} `{!threadG} sp esr stub_handler_addr (offset : bv 64) :
   instr 29756 (Some a743c) -∗
   instr_body 0x7400 (spec sp stub_handler_addr offset esr).
 Proof.
+(*PROOF_START*)
   iIntros "[? [? [? [? [? [? [? [? [? [? [i1 [i2 [i3 [i4 [? ?]]]]]]]]]]]]]]]".
   iAssert (instr_body 29736 (load_offset_spec offset 29752)) with "[i1 i2 i3 i4]" as "Hoffset".
   + iApply load_offset_verif.
     iFrame.
   + iApply wp. iFrame.
+(*PROOF_END*)
+Qed.
+
+Lemma reset_wp `{!islaG Σ} `{!threadG} :
+  instr 98888 (Some a18248) ∗
+  instr 98892 (Some a1824c) ∗
+  instr 98896 (Some a18250) ∗
+  instr 98900 (Some a18254) ∗
+  instr 98904 (Some a18258) ∗
+  instr 98908 (Some a1825c) ∗
+  instr 98912 (Some a18260) ∗
+  instr 98916 (Some a18264) ∗
+  instr 98920 (Some a18268) ∗
+  instr 98924 (Some a1826c) ∗
+  instr 98928 (Some a18270) ∗
+  instr 98932 (Some a18274) ∗
+  instr 98936 (Some a18278) ∗
+  instr 98940 (Some a1827c) ∗
+  instr 98944 (Some a18280) ∗
+  instr 98948 (Some a18284) -∗
+  instr_body 0x18248 reset_spec.
+Proof.
+(*PROOF_START*)
+  unfold reset_spec.
+  iStartProof.
+  do 500 liAStep; liShow.
+  liARun.
+  Unshelve.
+  all: prepare_sidecond.
+  all: try bv_solve.
+  + assert (Hshift: bv_shiftr spsr [BV{32} 0] = spsr); [by bits_simplify|].
+    rewrite Hshift.
+    rewrite H0.
+    by bits_simplify.
+  + bits_simplify.
+    bitify_hyp H4.
+    specialize (H4 n44 ltac:(lia)).
+    bits_simplify_hyp H4.
+    rewrite <- H4.
+    f_equal.
+    lia.
+(*PROOF_END*)
+Qed.
+
+
+
+Lemma stub_handler_wp `{!islaG Σ} `{!threadG} :
+  instr 98840 (Some a18218) ∗
+  instr 98844 (Some a1821c) ∗
+  instr 98848 (Some a18220) ∗
+  instr 98852 (Some a18224) ∗
+  instr 98856 (Some a18228) ∗
+  instr 98860 (Some a1822c) ∗
+  instr 98864 (Some a18230) ∗
+  instr 98868 (Some a18234) ∗
+  instr 98872 (Some a18238) ∗
+  instr 98876 (Some a1823c) ∗
+  instr 98880 (Some a18240) ∗
+  instr 98884 (Some a18244) ∗
+  instr_body 0x18248 reset_spec ∗
+  instr 98952 (Some a18288) ∗
+  instr 98956 (Some a1828c) ∗
+  instr 98960 (Some a18290) -∗
+  instr_body 0x18218 (stub_handler_spec).
+Proof.
+(*PROOF_START*)
+  unfold stub_handler_spec.
+  iStartProof.
+  liARun.
+  + unfold reset_spec.
+    liARun.
+  + (* This branch is a contradiction, but for now just let the proof proceed and contradict it later? *)
+    unfold reset_spec.
+    liARun.
+  Unshelve.
+  all: prepare_sidecond.
+  all: try bv_solve.
+  * assert (Hshift: bv_shiftr spsr [BV{32} 0] = spsr); [by bits_simplify|].
+    rewrite Hshift.
+    rewrite H0.
+    by bits_simplify.
+  * bits_simplify.
+    bitify_hyp H4.
+    specialize (H4 n ltac:(lia)).
+    bits_simplify_hyp H4.
+    rewrite <- H4.
+    f_equal.
+    lia.
+(*PROOF_END*)
 Qed.
